<?xml version="1.0" encoding="UTF-8"?>

<section xml:id="sec-lecture-5" xmlns:xi="http://www.w3.org/2001/XInclude">
  <title>Lecture 5 - Wave equation on the line </title>
  <introduction>
    <p> In this section, we'll solve the wave equation in the general case. We start here because the operator that defines the wave equation has very nice algebraic properties. </p>
    </introduction>
  <subsection xml:id="subsec-Solution">
    <title>Solution by factoring the operator</title>
    <p>Consider the equation
      <me>
        u_t - c^2 u_{xx}
      </me>
      where <m>x \in (-\infty, \infty)</m>.
      Writing this in operator form, we have
      <me>
        (\partial_t^2 - c^2 \partial_x^2)u = 0
      </me>
      which factors as 
      <me>
        (\partial_t - c\partial_x)(\partial_t + c\partial_x)u=0.
      </me>
      There are two ways that this equation can hold for a function <m>u</m>. The first is that <m>(\partial_t + c\partial_x)u = 0</m>. Solving
      <me>
        u_t + c u_x = 0,
      </me>
      note that <m>u</m> must be constant on lines parallel to the vector <m>(1, c)</m>, which means <m>u</m> is constant along lines of the form <m>x - ct = \xi</m> for constants <m>\xi</m>. As we've seen in earlier sections, this mean that such functions <m>u</m> must take the form <m>u(x,t) = f(x - ct)</m> for some arbitrary function <m>f</m>.
    </p>

    <p>The other possibility is that <m>(\partial_t + c\partial_x)u = v</m> for some non-zero function <m>v</m> in which case we need to solve the equation
      <me>
         (\partial_t - c\partial_x)(\partial_t + c\partial_x)u= (\partial_t - c\partial_x)v =0
      </me>
      Following the same idea as before, we conclude that <m>v = g(x + ct)</m> for some arbitrary function <m>v</m>. Of course, we aren't done, as we seek solutions <m>u</m>. That is, we must now solve the equation
      <me>
        (\partial_t + c\partial_x)u = v = g(x + ct)
      </me>
      which is equivalent to
      <me>
        u_t + c u_x = g(x + ct).
      </me>
      Note that if <m>u = G(x + ct)</m> where <m>G'(x) = \frac{1}{2c} g(x)</m>, then 
      <me>
        u_t + c u_x = G'(x+ct)(c) + c G'(x+ct)(1) = 2c G'(x + ct) = g(x+ ct),
      </me>
      and hence <m>u(x,t) = G(x+ct)</m> solves <m> (\partial_t + c\partial_x)u = v</m>. Then the general solution to the differential equation is of the form of a linear combination of our two arbitrary solutions:
      <me>
        u(x,t) = f(x - ct) + G(x + ct).
      </me>
    </p>
    <p> Right away, we can interpret what this means. The solutions to the wave equation on the line correspond to functions <m>f, g</m> traveling in opposite directions on the line as time tends from <m>0</m> to <m>\infty</m>. A Desmos workbook with some demonstration solutions can be found <url href="https://www.desmos.com/calculator/obytg6nbpj">here.</url>
    </p>
  </subsection>

</section>